theories/Prelude/PreludeInit.v
@@ -386,15 +386,9 @@ Module PreludeInit_MAIN.
 
   Context {dom : Hask.t} {cod : Hask.t}.
 
-  Definition im_eqProp {cod_isSetoid : isSetoid cod} (f : Hask.arrow dom cod) (lhs : dom) (rhs : dom) : Prop := binary_relation_on_image eqProp f lhs rhs.
-
-  Definition im_leProp {cod_isPoset : isPoset cod} (f : Hask.arrow dom cod) (lhs : dom) (rhs : dom) : Prop := binary_relation_on_image leProp f lhs rhs.
-
-  Variable f : Hask.arrow dom cod.
-
-  Local Instance equivalence_relation_on_image
-    (cod_isSetoid : isSetoid cod)
-    : Equivalence (im_eqProp f).
+  Local Instance relation_on_image_liftsEquivalence {eq_cod : cod -> cod -> Prop} (f : dom -> cod)
+    (requiresEquivalence : Equivalence eq_cod)
+    : Equivalence (binary_relation_on_image eq_cod f).
   Proof.
     constructor.
     - intros x1. exact (Equivalence_Reflexive (f x1)).
@@ -402,18 +396,20 @@ Module PreludeInit_MAIN.
     - intros x1 x2 x3 H_1EQ2 H_2EQ3. exact (Equivalence_Transitive (f x1) (f x2) (f x3) H_1EQ2 H_2EQ3).
   Defined.
 
-  Local Instance preorder_relation_on_image
-    (cod_isPoset : isPoset cod)
-    : PreOrder (im_leProp f).
+  Local Instance relation_on_image_liftsPreOrder {le_cod : cod -> cod -> Prop} (f : dom -> cod)
+    (requiresPreOrder : PreOrder le_cod)
+    : PreOrder (binary_relation_on_image le_cod f).
   Proof.
     constructor.
     - intros x1. exact (PreOrder_Reflexive (f x1)).
     - intros x1 x2 x3 H_1LE2 H_2LE3. exact (PreOrder_Transitive (f x1) (f x2) (f x3) H_1LE2 H_2LE3).
   Defined.
 
-  Local Instance partialorder_relation_on_image
-    (cod_isPoset : isPoset cod)
-    : PartialOrder (im_eqProp f) (im_leProp f).
+  Local Instance relation_on_image_liftsPartialOrder {eq_cod : cod -> cod -> Prop} {le_cod : cod -> cod -> Prop} (f : dom -> cod)
+    {requiresEquivalence : Equivalence eq_cod}
+    {requiresPreOrder : PreOrder le_cod}
+    (requiresPartialOrder : PartialOrder eq_cod le_cod)
+    : PartialOrder (binary_relation_on_image eq_cod f) (binary_relation_on_image le_cod f).
   Proof.
     intros x1 x2. constructor.
     - intros H_EQ. constructor.
@@ -423,6 +419,27 @@ Module PreludeInit_MAIN.
       + exact (proj1 H_EQ).
       + exact (proj2 H_EQ).
   Defined.
+
+  Definition im_eqProp {cod_isSetoid : isSetoid cod} (f : Hask.arrow dom cod) (lhs : dom) (rhs : dom) : Prop := binary_relation_on_image eqProp f lhs rhs.
+
+  Definition im_leProp {cod_isPoset : isPoset cod} (f : Hask.arrow dom cod) (lhs : dom) (rhs : dom) : Prop := binary_relation_on_image leProp f lhs rhs.
+
+  Variable f : Hask.arrow dom cod.
+
+  Local Instance equivalence_relation_on_image
+    (cod_isSetoid : isSetoid cod)
+    : Equivalence (im_eqProp f).
+  Proof. exact (relation_on_image_liftsEquivalence f eqProp_Equivalence). Defined.
+
+  Local Instance preorder_relation_on_image
+    (cod_isPoset : isPoset cod)
+    : PreOrder (im_leProp f).
+  Proof. exact (relation_on_image_liftsPreOrder f leProp_PreOrder). Defined.
+
+  Local Instance partialorder_relation_on_image
+    (cod_isPoset : isPoset cod)
+    : PartialOrder (im_eqProp f) (im_leProp f).
+  Proof. exact (relation_on_image_liftsPartialOrder f leProp_PartialOrder). Defined.
 
   End ImplFor_image.
 
